Trying Inductive contruction

Gratzer&Angiuli_Dependant_Types./Definitions.v
@@ -21,6 +21,80 @@ Inductive preContext : nat -> Type :=
 
 Notation "ctx # A" := (Extend ctx A) (at level 50, left associativity).
 
+Inductive wfContext : nat -> Type :=
+   I : wfContext 0
+| Extend_wf : forall {n}, wfContext n -> wfType n -> wfContext (S n)
+with wfType : nat -> Type :=
+  Base_wf : forall {n}, wfContext n -> wfType n
+| Func_wf : forall {n}, wfContext n -> wfType n -> wfType n -> wfType n
+| Prod_wf : forall {n}, wfContext n -> wfType n -> wfType n -> wfType n.
+Notation "⊢c ctx" := (ctx : wfContext) (at level 40).
+Notation "ctx ⊢t A" := (A : wfType) (at level 40).
+
+
+Fixpoint depth (A : preType) : nat :=
+  match A with
+  | Base => 0
+  | Func A B => Nat.max (depth A) (depth B) + 1
+  | Prod A B => Nat.max (depth A) (depth B) + 1
+  end.
+
+Fixpoint size {n} (ctx : preContext n) : nat :=
+  match ctx with
+  | Empty => 0
+  | Extend c T => size c + depth T
+  end.
+
+
+Fixpoint wfCtx {n} (ctx : preContext n) : Prop :=
+   match ctx with
+   | Empty => True
+   | Extend c T =>
+   let wfType' := fix wfType' (A : preType) : Prop :=
+      match A with
+      | Base => True
+      | Func A B => wfType' A /\ wfType' B
+      | Prod A B => wfType' A /\ wfType' B
+      end
+   in
+   wfCtx c /\ wfType' T
+end.
+Notation "⊢ ctx" := (wfCtx ctx) (at level 40).
+
+Fixpoint wfType {n} (ctx : preContext n) (W : ⊢ ctx) (A : preType) : Prop :=
+  match A with
+  | Base => True
+  | Func A B => wfType ctx W A /\ wfType ctx W B
+  | Prod A B => wfType ctx W A /\ wfType ctx W B
+  end.
+Notation "ctx ⊢ A 'ty'" := (wfType ctx _ A) (at level 40).
+
+
+Lemma base_well_formed : forall {n} (ctx : preContext n) (W : ⊢ ctx),
+  wfType ctx W Base.
+Proof.
+   simpl. auto.
+Qed.
+
+Lemma func_well_formed (A B : preType) : forall {n} (ctx : preContext n) (W : ⊢ ctx),
+   wfType ctx W A /\ wfType ctx W B -> wfType ctx W (A --> B).
+Proof.
+   simpl. auto.
+Qed.
+
+Lemma prod_well_formed (A B : preType) : forall {n} (ctx : preContext n) (W : ⊢ ctx),
+   wfType ctx W A /\ wfType ctx W B -> wfType ctx W (A ** B).
+Proof.
+   simpl. auto.
+Qed.
+
+
+Example ex1 : wfType Empty I ((Base ** Base) --> Base).
+Proof.
+  simpl. auto.
+Qed.
+
+
 Inductive preTerm :=
 | const (n : nat) : preTerm
 | Pair (a b : preTerm) : preTerm
@@ -28,3 +102,278 @@ Inductive preTerm :=
 | Snd (p : preTerm) : preTerm
 | Lam (b : preTerm) : preTerm
 | App (f a : preTerm) : preTerm.
+
+Fixpoint wfTerm {n} (ctx : preContext n) (A : preType) (t : preTerm) : Prop :=
+  match t,A with
+  | const _, Base => True
+  | Pair a b, A ** B => wfTerm ctx A a /\ wfTerm ctx B b
+  | Fst p, A => exists B, wfTerm ctx (A ** B) p
+  | Snd p, B => exists A, wfTerm ctx (A ** B) p
+  | Lam b, A --> B => wfTerm (ctx # A) B b
+  | App f a, B => exists A, wfTerm ctx (A --> B) f /\ wfTerm ctx A a
+  | _, _ => False
+  end.
+Notation "ctx ⊢ t ; A" := (wfTerm ctx A t) (at level 40).
+
+Fixpoint InContext (ctx : slContext) (x : slVariable) (t : slType) : Prop :=
+  match ctx with
+  | Empty => False
+  | Extend c y ty => if String.eqb x y then  ty = t else InContext c x t
+  end.
+
+Definition eq_ctx (ctx1 ctx2 : slContext) : Prop :=
+  forall x A, InContext ctx1 x A = InContext ctx2 x A.
+
+Lemma eq_ctx_refl (ctx : slContext) : eq_ctx ctx ctx.
+Proof.
+   intros. intros x A. reflexivity.
+Qed.
+
+Lemma eq_ctx_sym (ctx1 ctx2 : slContext) : eq_ctx ctx1 ctx2 -> eq_ctx ctx2 ctx1.
+Proof.
+   intros. intros x A. symmetry. apply H.
+Qed.
+
+Lemma eq_ctx_trans (ctx1 ctx2 ctx3 : slContext) :
+   eq_ctx ctx1 ctx2 -> eq_ctx ctx2 ctx3 -> eq_ctx ctx1 ctx3.
+Proof.
+   intros. intros x A. rewrite (H x A). apply H0.
+Qed.
+
+Add Relation slContext eq_ctx
+  reflexivity proved by eq_ctx_refl
+  symmetry proved by eq_ctx_sym
+  transitivity proved by eq_ctx_trans
+as eq_ctx_rel.
+
+Lemma ctx_extend_eq (ctx : slContext) (x : slVariable) (A B: slType) :
+   eq_ctx (Extend (Extend ctx x A) x B) (Extend ctx x B).
+Proof.
+   intros y C. simpl.
+   destruct (String.eqb y x) eqn:Heq;
+   reflexivity.
+Qed.
+
+
+
+Inductive slTerm :=
+| const : nat -> slTerm
+| Var : slVariable -> slTerm
+| Pair : slTerm -> slTerm -> slTerm
+| Fst : slTerm -> slTerm
+| Snd : slTerm -> slTerm
+| Lam (x : slVariable) (t : slTerm) : slTerm
+| App : slTerm -> slTerm -> slTerm.
+
+Fixpoint well_formed (ctx : slContext) (A : slType) (a : slTerm) : Prop :=
+  match a,A with
+  | const _, Base => True
+  | Var x, A => InContext ctx x A
+  | Pair t1 t2, A ** B => well_formed ctx A t1 /\ well_formed ctx B t2
+  | Fst t, A => exists B, well_formed ctx (A ** B) t
+  | Snd t, B => exists A, well_formed ctx (A ** B) t
+  | Lam x t, A --> B => well_formed (Extend ctx x A) B t
+  | App f a, B => exists A, well_formed ctx (A --> B) f /\ well_formed ctx A a
+  | _, _ => False
+  end.
+
+Notation "[ ctx ⊢ t ; A ]" := (well_formed ctx A t) (at level 40).
+
+
+Add Morphism well_formed with
+  signature eq_ctx ==> eq ==> eq ==> eq as well_formed_mor.
+Proof.
+   intros ctx1 ctx2 Hctx A a.
+   generalize dependent ctx2.
+   generalize dependent ctx1.
+   generalize dependent A.
+   generalize dependent a.
+   induction a; intros; simpl in *.
+   - reflexivity.
+   - apply Hctx.
+   - destruct A; try reflexivity.
+      rewrite (IHa1 A1 ctx1 ctx2 Hctx). rewrite (IHa2 A2 ctx1 ctx2 Hctx). reflexivity.
+   - f_equal.
+      apply functional_extensionality.
+      intros B.
+      apply IHa with (A:=A ** B); auto.
+   - f_equal.
+      apply functional_extensionality.
+      intros B.
+      apply IHa with (A:=B ** A); auto.
+   - destruct A; try reflexivity.
+      apply IHa.
+      unfold eq_ctx in *. intros y C.
+      simpl.
+      specialize (Hctx y C).
+      rewrite Hctx. reflexivity.
+   - f_equal.
+      apply functional_extensionality.
+      intros A0.
+      rewrite (IHa1 (A0 --> A) ctx1 ctx2 Hctx).
+      rewrite (IHa2 A0 ctx1 ctx2 Hctx).
+      reflexivity.
+Qed.
+
+
+Reserved Notation "b [ a // x ]" (at level 20).
+Fixpoint Subs (a b: slTerm)(x : slVariable) {struct b} : slTerm :=
+   match b with
+   | const n => const n
+   | Var y => if String.eqb y x then a else Var y
+   | Pair t1 t2 => Pair (t1 [ a // x ]) (t2 [ a // x ])
+   | Fst t => Fst (t [ a // x ])
+   | Snd t => Snd (t [ a // x ])
+   | Lam y t => if String.eqb x y then Lam y t else Lam y (t [ a // x ])
+   | App f t => App (f [ a // x ]) (t [ a // x ])
+   end
+where "b [ a // x ]" := (Subs a b x).
+
+Inductive eq_slTerm (ctx : slContext) (Ty : slType): relation slTerm :=
+| eq_refl : forall t : slTerm,
+    [ctx ⊢ t ; Ty] ->
+    eq_slTerm ctx Ty t t
+(* Beta_equivalence for Pairs *)
+| eq_beta_left : forall a b B, [ctx ⊢ a ; Ty] -> [ctx ⊢ b ; B] -> eq_slTerm ctx Ty (Fst (Pair a b)) a
+| eq_beta_right : forall a b A, [ctx ⊢ a ; A] ->  [ctx ⊢ b ; Ty] -> eq_slTerm ctx Ty (Snd (Pair a b)) b
+(* Eta_equivalence for Pairs *)
+| eq_eta_pair :
+   forall p A B, Ty = A ** B ->
+   [ctx ⊢ p ; Ty] -> eq_slTerm ctx Ty p (Pair (Fst p) (Snd p))
+(* Beta_equivalence for Lambdas *)
+| eq_beta_lam : forall t a x A,
+    [Extend ctx x A ⊢ t ; Ty] ->
+    [ctx ⊢ a ; A] ->
+    eq_slTerm ctx Ty (App (Lam x t) a) (t [ a // x ])
+(* Eta_equivalence for Lambdas *)
+| eq_eta_lam :
+   forall f x A B,
+   Ty = A --> B ->
+   [ctx ⊢ f ; Ty] ->
+    eq_slTerm ctx Ty f (Lam x (App f (Var x))).
+
+Axiom eq_slTerm_refl : forall (ctx : slContext) (A : slType),
+    reflexive slTerm (eq_slTerm ctx A).
+Axiom eq_slTerm_sym : forall (ctx : slContext) (A : slType),
+    symmetric slTerm (eq_slTerm ctx A).
+Axiom eq_slTerm_tans : forall (ctx : slContext) (A : slType),
+    transitive slTerm (eq_slTerm ctx A).
+
+Add Parametric Relation (ctx : slContext) (A : slType) : slTerm (eq_slTerm ctx A)
+  reflexivity proved by (eq_slTerm_refl ctx A)
+  symmetry proved by (eq_slTerm_sym ctx A)
+  transitivity proved by (eq_slTerm_tans ctx A)
+as eq_slTerm_rel.
+
+Notation "[ ctx ⊢ t1 '==' t2 ';' A ]" := (eq_slTerm ctx A t1 t2) (at level 40).
+
+
+Lemma Shadowing (ctx : slContext) (a : slTerm) (A C: slType) (x : slVariable) (B : slType) :
+   [Extend ctx x B ⊢ a ; C] = [Extend (Extend ctx x A) x B ⊢ a ; C].
+Proof.
+   apply well_formed_mor.
+   apply eq_ctx_sym.
+   apply ctx_extend_eq.
+   reflexivity.
+   reflexivity.
+Qed.
+
+Instance Proper_eq_slTerm : subrelation eq (impl).
+Proof.
+   intros a b H.
+   intros ctx.
+   subst.
+   auto.
+Qed.
+
+(* Lemma well_formed_extension (ctx : slContext) (a : slTerm) (A B : slType) (x : slVariable) :
+   [ctx ⊢ a ; A] -> [Extend ctx x B ⊢ a ; A].
+Proof.
+   intros H.
+   induction a; simpl in *; try assumption. *)
+
+
+Lemma Substitution (ctx : slContext) (a b : slTerm) (A B : slType) (x : slVariable) :
+   [Extend ctx x A ⊢ b ; B] /\ [ctx ⊢ a ; A] -> [ctx ⊢ (b [ a // x ]) ; B].
+Proof.
+   generalize dependent B.
+   generalize dependent A.
+   generalize dependent a.
+   generalize dependent ctx.
+   generalize dependent b.
+   induction b;
+   intros ctx a A B H;
+   destruct H as [H1 H2]; auto.
+   - simpl in *.
+    destruct (String.eqb s x) eqn:Heq; subst; auto.
+   - simpl in *. destruct B; try contradiction.
+     destruct H1 as [Hl Hr].
+     split; [ apply IHb1 with (A:=A) | apply IHb2 with (A:=A)]; auto.
+   - simpl in *. destruct H1 as [C Ht].
+       exists C. apply IHb with (A:=A); auto.
+   - simpl in *. destruct H1 as [C Ht].
+       exists C. apply IHb with (A:=A); auto.
+   - simpl in H1. destruct B; try contradiction.
+         simpl in *.
+         destruct (String.eqb x x0) eqn:Heq; subst;
+         simpl in *.
+         +
+         apply String.eqb_eq in Heq. subst.
+         rewrite Shadowing with (A:=A). apply H1.
+         +
+         apply String.eqb_neq in Heq.
+         apply IHb with (A:=A); auto.
+         split.
+         setoid_rewrite well_formed_mor in H1.
+         apply H1.
+         unfold eq_ctx.
+         intros. simpl.
+         destruct (String.eqb x1 x0) eqn:Heq1;
+         destruct (String.eqb x1 x) eqn:Heq2; try reflexivity.
+         apply String.eqb_eq in Heq1;
+           apply String.eqb_eq in Heq2; subst; contradiction.
+         reflexivity.
+         reflexivity.
+         (* Need the FreeVariable def to continue*)
+         admit.
+   - simpl in *. destruct H1 as [A' [Ht1 Ht2]].
+         exists A'. split;
+         [ apply IHb1 with (A:=A) | apply IHb2 with (A:=A)]; auto.
+Admitted.
+
+
+Instance Proper_Fst_eq (ctx : slContext) (A : slType) : Morphisms.Proper (eq_slTerm ctx A ==> eq) Fst.
+Proof.
+   intros a b H.
+   inversion H; subst; simpl; try reflexivity.
+Qed.
+
+Add Parametric Morphism (ctx : slContext) (A : slType) : (well_formed ctx A) with
+  signature (eq_slTerm ctx A) ==> eq as well_formed_eq_slTerm_mor.
+Proof.
+   induction A.
+   induction x, y; intro H; inversion H; subst; try contradiction; try reflexivity.
+   Set Rewrite Output Constraints.
+   - rewrite H.
+      all : shelve_unifiable.
+      all : try typeclasses eauto.
+   - apply Shadowing. auto.
+   - destruct H0 as [Hl Hr].
+     split; [ apply IHeq_slTerm1 | apply IHeq_slTerm2]; auto.
+   - destruct H0 as [B' Ht].
+       exists B'. apply IHeq_slTerm with (A:=A ** B'); auto.
+   - destruct H0 as [A' Ht].
+       exists A'. apply IHeq_slTerm with (A:=A --> B); auto.
+   - destruct H0 as [Hl Hr].
+     exists A0. split; [ apply IHeq_slTerm1 | apply IHeq_slTerm2]; auto.
+
+
+Lemma eq_slTerm_well_formed (ctx : slContext) (a b : slTerm) (A : slType) :
+   [ctx ⊢ a == b ; A] -> [ctx ⊢ a ; A] /\ [ctx ⊢ b ; A].
+Proof.
+   intros H.
+   inversion H; split; auto.
+   - setoid_rewrite eq_beta_left.
+      all : shelve_unifiable.
+      all : try typeclasses eauto.
+   simpl. exists B; auto.
